add: Log

Arithmetization/Exponential/Exp.lean
@@ -664,6 +664,11 @@ lemma monotone_iff {x₁ x₂ y₁ y₂ : M} (h₁ : Exp x₁ y₁) (h₂ : Exp 
   · exact monotone h₁ h₂
   · contrapose; simp; exact monotone_le h₂ h₁
 
+lemma monotone_le_iff {x₁ x₂ y₁ y₂ : M} (h₁ : Exp x₁ y₁) (h₂ : Exp x₂ y₂) : x₁ ≤ x₂ ↔ y₁ ≤ y₂ := by
+  constructor
+  · exact monotone_le h₁ h₂
+  · contrapose; simp; exact monotone h₂ h₁
+
 lemma add_mul {x₁ x₂ y₁ y₂ : M} (h₁ : Exp x₁ y₁) (h₂ : Exp x₂ y₂) : Exp (x₁ + x₂) (y₁ * y₂) := by
   wlog hy : y₁ ≥ y₂
   · simpa [add_comm, mul_comm] using this h₂ h₁ (le_of_not_ge hy)
@@ -682,149 +687,6 @@ lemma add_mul {x₁ x₂ y₁ y₂ : M} (h₁ : Exp x₁ y₁) (h₂ : Exp x₂ 
     simpa [←add_assoc, mul_left_comm y₁ 2 y₂] using exp_succ_mul_two.mpr this
 
 end Exp
-
-lemma log_exists_unique_pos {y : M} (hy : 0 < y) : ∃! x, x < y ∧ ∃ y' ≤ y, Exp x y' ∧ y < 2 * y' := by
-  have : ∃ x < y, ∃ y' ≤ y, Exp x y' ∧ y < 2 * y' := by
-    revert hy
-    induction y using hierarchy_polynomial_induction_sigma₀
-    · definability
-    case zero => simp
-    case even y IH =>
-      intro hy
-      rcases (IH (by simpa using hy) : ∃ x < y, ∃ y' ≤ y, Exp x y' ∧ y < 2 * y') with ⟨x, hxy, y', gey, H, lty⟩
-      exact ⟨x + 1, lt_of_lt_of_le (by simp [hxy]) (succ_le_double_of_pos (pos_of_gt hxy)),
-        2 * y', by simpa using gey, Exp.exp_succ_mul_two.mpr H, by simpa using lty⟩
-    case odd y IH =>
-      intro hy
-      rcases (zero_le y : 0 ≤ y) with (rfl | pos)
-      · simp; exact ⟨1, by simp [one_lt_two]⟩
-      · rcases (IH pos : ∃ x < y, ∃ y' ≤ y, Exp x y' ∧ y < 2 * y') with ⟨x, hxy, y', gey, H, lty⟩
-        exact ⟨x + 1, by simp; exact lt_of_lt_of_le hxy (by simp),
-          2 * y', le_trans (by simpa using gey) le_self_add, Exp.exp_succ_mul_two.mpr H, two_mul_add_one_lt_two_mul_of_lt lty⟩
-  rcases this with ⟨x, hx⟩
-  exact ExistsUnique.intro x hx (fun x' ↦ by
-    intro hx'
-    by_contra A
-    wlog lt : x < x'
-    · exact this hy x' hx' x hx (Ne.symm A) (lt_of_le_of_ne (by simpa using lt) A)
-    rcases hx with ⟨_, z, _, H, hyz⟩
-    rcases hx' with ⟨_, z', hzy', H', _⟩
-    have : z < z' := Exp.monotone H H' lt
-    have : y < y := calc
-      y < 2 * z := hyz
-      _ ≤ z'    := (Pow2.lt_iff_two_mul_le H.range_pow2 H'.range_pow2).mp this
-      _ ≤ y     := hzy'
-    simp at this)
-
-lemma log_exists_unique (y : M) : ∃! x, (y = 0 → x = 0) ∧ (0 < y → x < y ∧ ∃ y' ≤ y, Exp x y' ∧ y < 2 * y') := by
-  by_cases hy : y = 0
-  · rcases hy; simp
-  · simp [hy, pos_iff_ne_zero.mpr hy, log_exists_unique_pos]
-
-def log (a : M) : M := Classical.choose! (log_exists_unique a)
-
-@[simp] lemma log_zero : log (0 : M) = 0 :=
-  (Classical.choose!_spec (log_exists_unique (0 : M))).1 rfl
-
-lemma log_pos {y : M} (pos : 0 < y) : ∃ y' ≤ y, Exp (log y) y' ∧ y < 2 * y' :=
-  ((Classical.choose!_spec (log_exists_unique y)).2 pos).2
-
-lemma log_lt_self_of_pos {y : M} (pos : 0 < y) : log y < y :=
-  ((Classical.choose!_spec (log_exists_unique y)).2 pos).1
-
-@[simp] lemma log_le_self (a : M) : log a ≤ a := by
-  rcases zero_le a with (rfl | pos)
-  · simp
-  · exact le_of_lt <| log_lt_self_of_pos pos
-
-lemma log_graph {x y : M} : x = log y ↔ (y = 0 → x = 0) ∧ (0 < y → x < y ∧ ∃ y' ≤ y, Exp x y' ∧ y < 2 * y') := Classical.choose!_eq_iff _
-
-def logdef : Σᴬ[0] 2 := ⟨“(#1 = 0 → #0 = 0) ∧ (0 < #1 → #0 < #1 ∧ ∃[#0 < #2 + 1] (!Exp.def [#1, #0] ∧ #2 < 2 * #0))”, by simp⟩
-
-lemma log_defined : Σᴬ[0]-Function₁ (log : M → M) logdef := by
-  intro v; simp [logdef, log_graph, Exp.defined.pval, ←le_iff_lt_succ]
-
-instance {b s} : DefinableFunction₁ b s (log : M → M) := defined_to_with_param₀ _ log_defined
-
-instance : PolyBounded₁ (log : M → M) := ⟨#0, λ _ ↦ by simp⟩
-
-lemma log_eq_of_pos {x y : M} (pos : 0 < y) {y'} (H : Exp x y') (hy' : y' ≤ y) (hy : y < 2 * y') : log y = x :=
-  (log_exists_unique_pos pos).unique ⟨log_lt_self_of_pos pos, log_pos pos⟩ ⟨lt_of_lt_of_le H.dom_lt_range hy', y', hy', H, hy⟩
-
-@[simp] lemma log_one : log (1 : M) = 0 := log_eq_of_pos (by simp) (y' := 1) (by simp) (by rfl) (by simp [one_lt_two])
-
-lemma log_two_mul_of_pos {y : M} (pos : 0 < y) : log (2 * y) = log y + 1 := by
-  rcases log_pos pos with ⟨y', hy', H, hy⟩
-  exact log_eq_of_pos (by simpa using pos) (Exp.exp_succ_mul_two.mpr H) (by simpa using hy') (by simpa using hy)
-
-lemma log_two_mul_add_one_of_pos {y : M} (pos : 0 < y) : log (2 * y + 1) = log y + 1 := by
-  rcases log_pos pos with ⟨y', hy', H, hy⟩
-  exact log_eq_of_pos (by simp) (Exp.exp_succ_mul_two.mpr H)
-    (le_trans (by simpa using hy') le_self_add) (two_mul_add_one_lt_two_mul_of_lt hy)
-
-lemma log_eq_of_exp {x y : M} (H : Exp x y) : log y = x :=
-  log_eq_of_pos H.range_pos H (by { rfl }) (lt_mul_of_pos_of_one_lt_left H.range_pos one_lt_two)
-
-lemma exp_of_pow2 {p : M} (pp : Pow2 p) : Exp (log p) p := by
-  rcases log_pos pp.pos with ⟨q, hq, H, hp⟩
-  suffices : p = q
-  · simpa [this] using H
-  by_contra ne
-  have : q < p := lt_of_le_of_ne hq (Ne.symm ne)
-  have : 2 * q < 2 * q := calc
-    2 * q ≤ p     := (Pow2.lt_iff_two_mul_le H.range_pow2 pp).mp this
-    _     < 2 * q := hp
-  simp at this
-
-lemma log_mul_pow2 {a p : M} (pos : 0 < a) (pp : Pow2 p) : log (a * p) = log a + log p := by
-  rcases log_pos pos with ⟨a', ha', Ha, ha⟩
-  rcases log_pos pp.pos with ⟨p', hp', Hp, hp⟩
-  exact log_eq_of_pos (mul_pos pos pp.pos) (Exp.add_mul Ha Hp) (mul_le_mul' ha' hp') (by
-    rcases Hp.uniq (exp_of_pow2 pp)
-    simp [←mul_assoc]; exact mul_lt_mul_of_pos_right ha pp.pos)
-
-def binaryLength (a : M) : M := if 0 < a then log a + 1 else 0
-
-notation "‖" a "‖" => binaryLength a
-
-@[simp] lemma binary_length_zero : ‖(0 : M)‖ = 0 := by simp [binaryLength]
-
-lemma binary_length_of_pos {a : M} (pos : 0 < a) : ‖a‖ = log a + 1 := by simp [binaryLength, pos]
-
-@[simp] lemma binary_length_le (a : M) : ‖a‖ ≤ a := by
-  rcases zero_le a with (rfl | pos)
-  · simp
-  · simp [pos, binary_length_of_pos, ←lt_iff_succ_le, log_lt_self_of_pos]
-
-lemma binary_length_graph {i a : M} : i = ‖a‖ ↔ (0 < a → ∃ k ≤ a, k = log a ∧ i = k + 1) ∧ (a = 0 → i = 0) := by
-  rcases zero_le a with (rfl | pos)
-  · simp
-  · simp [binary_length_of_pos, pos, pos_iff_ne_zero.mp pos]
-    constructor
-    · rintro rfl; exact ⟨log a, by simp⟩
-    · rintro ⟨_, _, rfl, rfl⟩; rfl
-
-def binarylengthdef : Σᴬ[0] 2 := ⟨“(0 < #1 → ∃[#0 < #2 + 1] (!logdef [#0, #2] ∧ #1 = #0 + 1)) ∧ (#1 = 0 → #0 = 0)”, by simp⟩
-
-lemma binary_length_defined : Σᴬ[0]-Function₁ (binaryLength : M → M) binarylengthdef := by
-  intro v; simp [binarylengthdef, binary_length_graph, log_defined.pval, ←le_iff_lt_succ]
-
-instance {b s} : DefinableFunction₁ b s (binaryLength : M → M) := defined_to_with_param₀ _ binary_length_defined
-
-instance : PolyBounded₁ (binaryLength : M → M) := ⟨#0, λ _ ↦ by simp⟩
-
-@[simp] lemma binary_length_one : ‖(1 : M)‖ = 1 := by simp [binaryLength]
-
-lemma binary_length_two_mul_of_pos {a : M} (pos : 0 < a) : ‖2 * a‖ = ‖a‖ + 1 := by
-  simp [pos, binary_length_of_pos, log_two_mul_of_pos]
-
-lemma binary_length_two_mul_add_one (a : M) : ‖2 * a + 1‖ = ‖a‖ + 1 := by
-  rcases zero_le a with (rfl | pos)
-  · simp
-  · simp [pos, binary_length_of_pos, log_two_mul_add_one_of_pos]
-
-lemma binary_length_mul_pow2 {a p : M} (pos : 0 < a) (pp : Pow2 p) : ‖a * p‖ = ‖a‖ + log p := by
-  simp [binary_length_of_pos, pos, pp.pos, log_mul_pow2 pos pp, add_right_comm (log a) (log p) 1]
 
 end ISigma₀
 
@@ -890,19 +752,8 @@ lemma exp_even (a : M) : exp (2 * a) = (exp a)^2 :=
 @[simp] lemma exponential_monotone {a b : M} : exp a < exp b ↔ a < b :=
   Iff.symm <| Exp.monotone_iff (exp_exponential a) (exp_exponential b)
 
-@[simp] lemma log_exponential (a : M) : log (exp a) = a := log_eq_of_exp (exp_exponential a)
-
-@[simp] lemma binary_length_exponential (a : M) : ‖exp a‖ = a + 1 := by
-  simp [binary_length_of_pos]
-
-lemma exp_add (a b : M) : exp (a + b) = exp a * exp b :=
-  exponential_of_exp (Exp.add_mul (exp_exponential a) (exp_exponential b))
-
-lemma log_mul_exp {a : M} (pos : 0 < a) (i : M) : log (a * exp i) = log a + i := by
-  simp [log_mul_pow2 pos (exp_pow2 i)]
-
-lemma binary_length_mul_exp {a : M} (pos : 0 < a) (i : M) : ‖a * exp i‖ = ‖a‖ + i := by
-  simp [binary_length_mul_pow2 pos (exp_pow2 i)]
+@[simp] lemma exponential_monotone_le {a b : M} : exp a ≤ exp b ↔ a ≤ b :=
+  Iff.symm <| Exp.monotone_le_iff (exp_exponential a) (exp_exponential b)
 
 end exponential
 
